compiler/dsl/coq/ReflexQuark.v
@@ -18,10 +18,6 @@ Definition splitAt c s :=
     end
   in splitAt_aux c s nil.
 
-Definition dom s :=
-  let url_end := snd (splitAt "." s) in
-  fst (splitAt "/" url_end).
-
 Open Scope string_scope.
 
 Module SystemFeatures <: SystemFeaturesInterface.
@@ -95,6 +91,11 @@ Module Spec <: SpecInterface.
 
 Include SystemFeatures.
 
+Open Scope char_scope.
+Definition dom {term} s :=
+  (splitfst term "/" (splitsnd term "." s)).
+Close Scope char_scope.
+
 Definition INIT : init_prog PAYD COMPT COMPS KSTD IENVD :=
   seq (spawn IENVD _ Output    tt                   i_output    (Logic.eq_refl _)) (
   seq (spawn IENVD _ Tab       (default_domain, tt) i_curtab    (Logic.eq_refl _)) (
@@ -104,89 +105,46 @@ Definition INIT : init_prog PAYD COMPT COMPS KSTD IENVD :=
   seq (stupd IENVD _ v_curtab (Term _ (base_term _ IENVD) (Var _ IENVD i_curtab))
   ) nop))))).
 
-(*
-                        (
-                          shvec_ith (n := (projT1 (compd_conf (COMPS Tab))))
-                            sdenote_desc
-                            (projT2 (compd_conf (COMPS Tab)))
-                            (comp_conf (st0##v_curtab%kst))
-                            None
-                        )
-*)
-
-Print comp.
-
+Open Scope hdlr.
 Definition HANDLERS : handlers PAYD COMPT COMPS KSTD :=
-  fun m cc =>
-  let (ct, cf, ccf) := cc in
-  match m as _m return forall (EQ : _m = m), _ with
-  | {| tag := t; pay := p |} =>
+  fun t ct =>
   match ct as _ct, t as _t return
-    forall _p, Build_msg PAYD _t _p = m -> s[[ comp_conf_desc _ _ _ct ]] -> _
+    {prog_envd : vcdesc COMPT & hdlr_prog PAYD COMPT COMPS KSTD prog_envd _ct _t}
   with
-
   | _, Some (Some (Some (Some (Some (Some (Some (Some (Some (Some bad))))))))) =>
     match bad with end
 
-  | Tab, ReqSocket => fun pl EQ ccf =>
-    let envd := mk_vcdesc [] in
-    match pl with (url, _) =>
-    existT (fun d => hdlr_prog PAYD COMPT COMPS KSTD cc m d) envd
-    (
-      ite envd _ (
-            BinOp _ _
-                  (Eq _ (Desc _ fd_d))
-                  (Term _ _ (CompFd _ _ ccomp))
-                  (Term _ _ (CompFd _ _ (stvar v_curtab)))
-          )
-      (
-        ite envd _ (BinOp _ _
-                      (Eq _ (Desc _ str_d))
-                      (slit (dom url))
-                      (cconf (cc:= Build_comp SystemFeatures.COMPT SystemFeatures.COMPS Tab cf ccf) 0%fin)
-                   )
-        (
-          nop
-        )
-        (
-          nop
-        )
-      )
-      (
-        nop
-      )
-    )
-    end
-
-  | UserInput, KeyPress => fun pl EQ ccf =>
-    let envd := mk_vcdesc [] in
-    match pl with (key, _) =>
-    existT (fun d => hdlr_prog PAYD COMPT COMPS KSTD cc m d) envd
-    (
-      seq (send envd _ _ (stvar v_curtab) KeyPress (slit key, tt))
-      nop
-    )
-    end
-
-  | UserInput, MouseClick => fun pl EQ ccf =>
-    let envd := mk_vcdesc [] in
-    match pl with (pos, _) =>
-    existT (fun d => hdlr_prog PAYD COMPT COMPS KSTD cc m d) envd
-    (
-      seq (send envd _ _ (stvar v_curtab) MouseClick (slit pos, tt))
-      nop
-    )
-    end
-
-  | _, _ => fun _ _ _ =>
-    let envd := mk_vcdesc [] in
-    existT (fun d => hdlr_prog PAYD COMPT COMPS KSTD cc m d) envd
-    nop
-
-  end p
-  end (Logic.eq_refl m).
-
-Definition HANDLERS : handlers PAYD COMPT COMPS KSTD :=
+  | Tab, ReqSocket =>
+    [[ mk_vcdesc [] :
+        ite (eq ccomp (stvar v_curtab))
+            (
+              (*This should really compare the domain of the message to the
+                domain of the tab.*)
+              ite (eq (dom (mvar ReqSocket None)) (cconf Tab None))
+                  (
+                    nop
+                  )
+                  (
+                    nop
+                  )
+            ) 
+            ( 
+              nop
+            )
+    ]]
+  | UserInput, KeyPress =>
+      [[ mk_vcdesc [] :
+      seq (send (stvar v_curtab) KeyPress (mvar KeyPress None, tt))
+      nop ]]
+  | UserInput, MouseClick =>
+      [[ mk_vcdesc [] :
+      seq (send (stvar v_curtab) MouseClick (mvar MouseClick None, tt))
+      nop ]]
+  | _, _ =>
+    [[ mk_vcdesc [] : nop ]]
+  end.
+Close Scope hdlr.
+(*Definition HANDLERS : handlers PAYD COMPT COMPS KSTD :=
   (fun m cc =>
      let (ct, cf, cconf) := cc in
      match ct, tag PAYD m as _tm return
@@ -260,7 +218,7 @@ Definition HANDLERS : handlers PAYD COMPT COMPS KSTD :=
 
     end (pay PAYD m)
   ).
-
+*)
 End Spec.
 
 Module Main := MkMain(Spec).
